redefined as inductive, defined reset group and close group, added validity invariant

vt/PikeVM_VT.v
@@ -34,7 +34,7 @@ and blocked thread, we can do the "acceleration" step, where we jump ahead in th
 to the next position where the prefix matches.
 *)
 
-From Stdlib Require Import List Lia.
+From Stdlib Require Import List Lia Permutation.
 Import ListNotations.
 From Stdlib Require Import Program.Equality.
 
@@ -55,145 +55,159 @@ Section PikeVM_VT.
   Context {VMS: VMSeen}.
   Context (rer: RegExpRecord).
 
-(** * Registers *)
+  (** * Registers *)
 
   Definition regs := Regs.State.
   Definition regs_id := nat. (* virtual tree leaf id *)
   Definition gid_to_idx (gid:group_id) : nat := 2 * gid.
 
-  (** * PikeVM threads  *)
+  (** * PikeVM_VT threads  *)
   
-Definition thread_vt : Type := (label * regs_id * LoopBool).
+  Definition thread_vt : Type := (label * regs_id * LoopBool).
 
-Definition upd_label_vt (t:thread_vt) (next:label) (ri:regs_id) : thread_vt :=
-  match t with (l,r,b) => (next,ri,b) end.
+  Definition upd_label_vt (t:thread_vt) (next:label) (ri:regs_id) : thread_vt :=
+    match t with (l,r,b) => (next,ri,b) end.
 
-Definition advance_thread_vt (t:thread_vt) : thread_vt :=
-  match t with (l,r,b) => (l+1,r,b) end.
+  Definition advance_thread_vt (t:thread_vt) : thread_vt :=
+    match t with (l,r,b) => (l+1,r,b) end.
 
-(* used after consuming *)
-Definition block_thread_vt (t:thread_vt) : thread_vt :=
-  match t with (l,r,b) => (l+1,r,CanExit) end.
+  (* used after consuming *)
+  Definition block_thread_vt (t:thread_vt) : thread_vt :=
+    match t with (l,r,b) => (l+1,r,CanExit) end.
 
-Definition open_thread_vt (t:thread_vt) (gid:group_id) (idx:nat) (r:regs): thread_vt * regs :=
-  match t with
-    (l,ri,b) =>
-      (* the third value in the triple is unused *)
-      let new_data := Incomplete([(gid_to_idx gid, Valid(idx), Undefined)]) in
-      let r' := Regs.insert ri new_data r in
-      ((l+1, ri, b), r') end.
+  Definition open_thread_vt (t:thread_vt) (gid:group_id) (idx:nat) (r:regs): thread_vt * regs :=
+    match t with
+      (l,ri,b) =>
+        (* the third value in the triple is unused *)
+        let new_data := Incomplete([(gid_to_idx gid, Valid(idx), Undefined)]) in
+        let r' := Regs.insert ri new_data r in
+        ((l+1, ri, b), r') end.
 
-Definition close_thread_vt (t:thread_vt) (gid:group_id) (idx:nat) (r:regs): thread_vt * regs :=
-  match t with
-    (l,ri,b) =>
-      (* the third value in the triple is unused *)
-      let new_data := Incomplete([(gid_to_idx gid + 1, Valid(idx), Undefined)]) in
-      let r' := Regs.insert ri new_data r in
-      ((l+1, ri, b), r') end.
-(* In GroupMap.close, if the opening value is greater than idx, then they are switched. 
-Should I do that ?
-TODO: get_compressed data on ri, get with gid_to_idx gid, if larger, add update for both regs *)
+  Definition close_thread_vt (t:thread_vt) (gid:group_id) (idx:nat) (r:regs): thread_vt * regs :=
+    match t with
+      (l,ri,b) =>
+        match Regs.get_compressed_data ri r with
+        | None => (t, r) (* does nothing when the group has not been opened *)
+        | Some regsdata =>
+            match get_at (gid_to_idx gid) 0 regsdata with
+            (* the second value is the unused clock *)
+            | (None, _) => (t, r) (* does nothing when the group has not been opened *)
+            | (Some startIdx, _) =>
+                if (startIdx <=? idx) then
+                  let new_close := Incomplete([(gid_to_idx gid + 1, Valid(idx), Undefined)]) in
+                  let r' := Regs.insert ri new_close r in
+                  ((l+1, ri, b), r')
+                else
+                  let new_start := Incomplete([(gid_to_idx gid, Valid(idx), Undefined)]) in
+                  let new_close := Incomplete([(gid_to_idx gid + 1, Valid(startIdx), Undefined)]) in
+                  let r' := Regs.insert ri new_start r in
+                  let r'' := Regs.insert ri new_close r' in
+                  ((l+1, ri, b), r'')
+            end
+        end
+    end.
 
-Definition reset_thread_vt (t:thread_vt) (gidl:list group_id) (r:regs): thread_vt * regs :=
-  match t with
-    (l,ri,b) =>
-      let r' := List.fold_left (fun r gid =>
-                        let new_data := Incomplete([]) in
-                        Regs.insert ri new_data r) gidl r in
-      ((l+1, ri, b), r') end.
+  Definition reset_thread_vt (t:thread_vt) (gidl:list group_id) (r:regs): thread_vt * regs :=
+    match t with
+      (l,ri,b) =>
+        let r' := List.fold_left (
+                      fun r gid =>
+                        let new_start := Incomplete([(gid_to_idx gid, Invalid, Undefined)]) in
+                        let new_close := Incomplete([(gid_to_idx gid + 1, Invalid, Undefined)]) in
+                        let r' := Regs.insert ri new_start r in
+                        Regs.insert ri new_close r')
+                    gidl r in
+        ((l+1, ri, b), r') end.
 
-Definition begin_thread_vt (t:thread_vt) : thread_vt :=
-  match t with (l,r,b) => (l+1,r,CannotExit) end.
+  Definition begin_thread_vt (t:thread_vt) : thread_vt :=
+    match t with (l,r,b) => (l+1,r,CannotExit) end.
+  
+  Definition ri_of (t:thread_vt) : regs_id :=
+    match t with (pc,ri,b) => ri end.
 
-(*Definition gm_of (t:thread_vt) : group_map :=
-  match t with (pc,gm,b) => gm end.*)
-Definition ri_of (t:thread_vt) : regs_id :=
-  match t with (pc,ri,b) => ri end.
+  Definition seen_thread_vt (seen:seenpcs) (t:thread_vt) :bool :=
+    match t with
+    | (pc, gm, b) => inseenpc seen pc b
+    end.
 
-Definition seen_thread_vt (seen:seenpcs) (t:thread_vt) :bool :=
-  match t with
-  | (pc, gm, b) => inseenpc seen pc b
-  end.
-
-Definition add_thread_vt (seen:seenpcs) (t:thread_vt) : seenpcs :=
-  match t with
-  | (pc, gm, b) => add_seenpcs seen pc b
-  end.
+  Definition add_thread_vt (seen:seenpcs) (t:thread_vt) : seenpcs :=
+    match t with
+    | (pc, gm, b) => add_seenpcs seen pc b
+    end.
 
 
-(** * NFA epsilon-exploration  *)
+  (** * NFA epsilon-exploration  *)
 
-(* the result of one step of exploring transitions *)
-Inductive epsilon_result_vt : Type :=
-| EpsActive_vt: list thread_vt -> epsilon_result_vt
-| EpsMatch_vt: epsilon_result_vt
-| EpsBlocked_vt: thread_vt -> epsilon_result_vt.
+  (* the result of one step of exploring transitions *)
+  Inductive epsilon_result_vt : Type :=
+  | EpsActive_vt: list thread_vt -> epsilon_result_vt
+  | EpsMatch_vt: epsilon_result_vt
+  | EpsBlocked_vt: thread_vt -> epsilon_result_vt.
 
-Definition EpsDead_vt : epsilon_result_vt := EpsActive_vt [].
+  Definition EpsDead_vt : epsilon_result_vt := EpsActive_vt [].
 
-(* an atomic step for a thread *)
-(* TODO add regs as input and output: so that we can insert/split/delete *)
-Definition epsilon_step_vt (t:thread_vt) (c:code) (i:input) (r:regs) : epsilon_result_vt * regs :=
-  match t with
-  | (pc, ri, b) =>
-      match get_pc c pc with
-      | None =>
-          let r' := Regs.delete ri r in
-          (EpsDead_vt, r')
-      | Some instr =>
-          match instr with
-          | Accept => (EpsMatch_vt, r)
-          | Consume cd => match check_read rer cd i forward with
-                          | CannotRead =>
-                              let r' := Regs.delete ri r in
-                              (EpsDead_vt, r')
-                          | CanRead => (EpsBlocked_vt (block_thread_vt t), r)
-                         end
-          | CheckAnchor a => match anchor_satisfied rer a i with
-                             | false =>
-                                 let r' := Regs.delete ri r in
-                                 (EpsDead_vt, r')
-                             | true => (EpsActive_vt [advance_thread_vt t], r)
-                             end
-          | Jmp next => (EpsActive_vt [upd_label_vt t next ri], r)
-          | Fork l1 l2 =>
-              let (r', ri') := (Regs.split ri r) in
-              (EpsActive_vt [upd_label_vt t l1 ri; upd_label_vt t l2 ri'], r')
-          | SetRegOpen gid =>
-              let (t', r') := open_thread_vt t gid (idx i) r in
-              (EpsActive_vt [t'], r')
-          | SetRegClose gid =>
-              let (t', r') := close_thread_vt t gid (idx i) r in
-              (EpsActive_vt [t'], r')
-          | ResetRegs gidl =>
-              let (t', r') := reset_thread_vt t gidl r in
-              (EpsActive_vt [t'], r')
-          | BeginLoop => (EpsActive_vt [begin_thread_vt t], r)
-          | EndLoop next => match b with
-                            | CannotExit =>
+  (* an atomic step for a thread *)
+  Definition epsilon_step_vt (t:thread_vt) (c:code) (i:input) (r:regs) : epsilon_result_vt * regs :=
+    match t with
+    | (pc, ri, b) =>
+        match get_pc c pc with
+        | None =>
+            let r' := Regs.delete ri r in
+            (EpsDead_vt, r')
+        | Some instr =>
+            match instr with
+            | Accept => (EpsMatch_vt, r)
+            | Consume cd => match check_read rer cd i forward with
+                            | CannotRead =>
                                 let r' := Regs.delete ri r in
                                 (EpsDead_vt, r')
-                            | CanExit => (EpsActive_vt [upd_label_vt t next ri], r)
+                            | CanRead => (EpsBlocked_vt (block_thread_vt t), r)
                             end
-          | KillThread =>
-              let r' := Regs.delete ri r in
-              (EpsDead_vt, r')
-          end
-      end
-  end.
+            | CheckAnchor a => match anchor_satisfied rer a i with
+                               | false =>
+                                   let r' := Regs.delete ri r in
+                                   (EpsDead_vt, r')
+                               | true => (EpsActive_vt [advance_thread_vt t], r)
+                               end
+            | Jmp next => (EpsActive_vt [upd_label_vt t next ri], r)
+            | Fork l1 l2 =>
+                let (r', ri') := (Regs.split ri r) in
+                (EpsActive_vt [upd_label_vt t l1 ri; upd_label_vt t l2 ri'], r')
+            | SetRegOpen gid =>
+                let (t', r') := open_thread_vt t gid (idx i) r in
+                (EpsActive_vt [t'], r')
+            | SetRegClose gid =>
+                let (t', r') := close_thread_vt t gid (idx i) r in
+                (EpsActive_vt [t'], r')
+            | ResetRegs gidl =>
+                let (t', r') := reset_thread_vt t gidl r in
+                (EpsActive_vt [t'], r')
+            | BeginLoop => (EpsActive_vt [begin_thread_vt t], r)
+            | EndLoop next => match b with
+                              | CannotExit =>
+                                  let r' := Regs.delete ri r in
+                                  (EpsDead_vt, r')
+                              | CanExit => (EpsActive_vt [upd_label_vt t next ri], r)
+                              end
+            | KillThread =>
+                let r' := Regs.delete ri r in
+                (EpsDead_vt, r')
+            end
+        end
+    end.
 
-(** * PikeVM Semantics  *)
+  (** * PikeVM_VT Semantics  *)
 
-Definition leaf_vt : Type := input * regs_id.
+  Definition leaf_vt : Type := input * regs_id.
 
-(* semantic states of the PikeVM algorithm *)
-Inductive pike_vm_state_vt : Type :=
-| PVS_vt (inp:input) (active: list thread_vt) (best: option leaf_vt) (blocked: list thread_vt) (nextprefix: option (nat * literal * StrSearch)) (seen: seenpcs) (r:regs)
-| PVS_final_vt (best: option leaf_vt) (r: regs).
+  (* semantic states of the PikeVM_VT algorithm *)
+  Inductive pike_vm_state_vt : Type :=
+  | PVS_vt (inp:input) (active: list thread_vt) (best: option leaf_vt) (blocked: list thread_vt) (nextprefix: option (nat * literal * StrSearch)) (seen: seenpcs) (r:regs)
+  | PVS_final_vt (best: option leaf_vt) (r: regs).
 
 (* given an input and literal, we compute the next prefix counter *)
 (* since the counter is always offset by one, we first try to advance the input before performing a prefix search *)
-Definition next_prefix_counter {strs:StrSearch} (inp: input) (lit: literal) : option (nat * literal * StrSearch) :=
+(*Definition next_prefix_counter {strs:StrSearch} (inp: input) (lit: literal) : option (nat * literal * StrSearch) :=
   match advance_input inp forward with
   | None => None
   | Some (Input next pref) =>
@@ -201,484 +215,642 @@ Definition next_prefix_counter {strs:StrSearch} (inp: input) (lit: literal) : op
       | None => None
       | Some n => Some (n, lit, strs)
       end
-  end.
-
-Definition vt_initial_id := 0.
-Definition pike_vm_initial_thread_vt : thread_vt := (0, vt_initial_id, CanExit).
-
-(* initial state for the PikeVM which operates in unanchored fashion *)
-(* ignored for vt *)
-(*Definition pike_vm_initial_state_unanchored {strs:StrSearch} (lit:literal) (inp:input) : pike_vm_state :=
-  let nextprefix := next_prefix_counter inp lit in
-  PVS inp [pike_vm_initial_thread] None [] nextprefix initial_seenpcs.*)
-
-(* initial state for the PikeVM which operates in anchored fashion *)
-Definition pike_vm_initial_state_vt (inp:input) (regs_size: nat) : pike_vm_state_vt :=
-  PVS_vt inp [pike_vm_initial_thread_vt] None [] None initial_seenpcs (Regs.initial_tree regs_size).
-
-Definition delete_thread_regs_from_regs_state: list thread_vt -> regs -> regs :=
-  List.fold_left (fun r t => (* get regs_id from thread, delete it from r *)
-                    match t with
-                      (_, ri, _) => Regs.delete ri r end).
-Definition delete_best_regs_from_regs_state (best:option leaf_vt) (r:regs) : regs :=
-  match best with
-  | Some (_, ri) => Regs.delete ri r
-  | None => r
-  end.
-
-(* small-step semantics for the PikeVM algorithm *)
-Inductive pike_vm_step_vt (c:code): pike_vm_state_vt -> pike_vm_state_vt -> Prop :=
-| pvs_final_vt:
-  (* moving to a final state when there are no more active or blocked threads *)
-  forall inp best seen regs,
-    pike_vm_step_vt c (PVS_vt inp [] best [] None seen regs) (PVS_final_vt best regs)
-| pvs_end_vt:
-  (* when the list of active is empty and we've reached the end of string *)
-  (* in practice, this rule is never used because we can have no blocked threads *)
-  (* when there is no input left. We keep this rule for convenience in the proofs *)
-  (* and for relating it to the functional version *)
-  forall inp best thr blocked nextprefix seen regs regs'
-         (ADVANCE: advance_input inp forward = None)
-         (DELETE_REGS: regs' = delete_thread_regs_from_regs_state (thr::blocked) regs),
-    pike_vm_step_vt c (PVS_vt inp [] best (thr::blocked) nextprefix seen regs)
-      (PVS_final_vt best regs')
-| pvs_nextchar_vt:
-  (* when the list of active threads is empty (but not blocked), restart from the blocked ones, proceeding to the next character *)
-  (* reset the set of seen pcs *)
-  forall inp1 inp2 best thr blocked seen regs
-         (ADVANCE: advance_input inp1 forward = Some inp2),
-    pike_vm_step_vt c (PVS_vt inp1 [] best (thr::blocked) None seen regs)
-      (PVS_vt inp2 (thr::blocked) best [] None initial_seenpcs regs)
-| pvs_skip_vt:
-  (* when the pc has already been seen at this current index, we skip it entirely *)
-  forall inp t active best blocked nextprefix seen regs regs'
-         (SEEN: seen_thread_vt seen t = true)
-         (DELETE_REG:  regs' = delete_thread_regs_from_regs_state [t] regs), (* t is killed, so its regs are deleted *)
-    pike_vm_step_vt c (PVS_vt inp (t::active) best blocked nextprefix seen regs)
-      (PVS_vt inp active best blocked nextprefix seen regs')
-| pvs_active_vt:
-  (* generated new active threads: add them in front of the low-priority ones *)
-  forall inp t active best blocked nextprefix seen nextactive regs regs'
-         (UNSEEN: seen_thread_vt seen t = false)
-         (STEP: epsilon_step_vt t c inp regs = (EpsActive_vt nextactive, regs')), (* returns next regs *)
-    pike_vm_step_vt c (PVS_vt inp (t::active) best blocked nextprefix seen regs)
-      (PVS_vt inp (nextactive++active) best blocked nextprefix (add_thread_vt seen t) regs')
-| pvs_match_vt:
-  (* a match is found, discard remaining low-priority active threads *)
-  forall inp t active best blocked nextprefix seen regs regs' regs''
-         (UNSEEN: seen_thread_vt seen t = false)
-         (STEP: epsilon_step_vt t c inp regs = (EpsMatch_vt, regs'))
-         (* delete regs of active threads (except t) and of previous best match *)
-         (DELETE_REGS: regs'' = delete_thread_regs_from_regs_state active
-                                  (delete_best_regs_from_regs_state best regs')),
-    pike_vm_step_vt c (PVS_vt inp (t::active) best blocked nextprefix seen regs) 
-      (PVS_vt inp [] (Some (inp,ri_of t)) blocked None (add_thread_vt seen t) regs'')
-| pvs_blocked_vt:
-  (* add the new blocked thread after the previous ones *)
-  forall inp t active best blocked nextprefix seen newt regs regs'
-         (UNSEEN: seen_thread_vt seen t = false)
-         (STEP: epsilon_step_vt t c inp regs = (EpsBlocked_vt newt, regs')), (* returns new regs *)
-    pike_vm_step_vt c (PVS_vt inp (t::active) best blocked nextprefix seen regs)
-      (PVS_vt inp active best (blocked ++ [newt]) nextprefix (add_thread_vt seen t) regs').
-(* Unanchored PikeVM rules are removed: pvs_acc, pvs_nextchar_generate, pvs_next_char_filter *)
-
-(** * Equivalence to the original PikeVM *)
-
-Definition trc_pike_vm_vt (c:code) := @trc pike_vm_state_vt (pike_vm_step_vt c).
-
-Definition rer_to_regs_size : nat :=
+  end.*)
+  Definition rer_to_regs_size : nat :=
   match rer with
   | RegExpRecord.make _ _ _ _ cgc => 2 * cgc (* regs_size = 2 * rer.capturingGroupsCount *)
   end.
+  
+  Definition vt_initial_id := 0.
+  Definition pike_vm_initial_thread_vt : thread_vt := (0, vt_initial_id, CanExit).
 
-Definition gm_regs_vals (gid: group_id) (gm: group_map) : option nat * option nat :=
-  match GroupMap.find gid gm with
-  | None => (None, None)
-  | Some (GroupMap.Range v None) => (Some v, None)
-  | Some (GroupMap.Range o (Some c)) => (Some o, Some c)
-  end.
+  (* initial state for the PikeVM_VT which operates in anchored fashion *)
+  Definition pike_vm_initial_state_vt (inp:input) (regs_size: nat) : pike_vm_state_vt :=
+    PVS_vt inp [pike_vm_initial_thread_vt] None [] None initial_seenpcs (Regs.initial_tree regs_size).
 
-Definition vt_regs_vals (gid: group_id) (regsdata: RegsData.t) : option nat * option nat :=
-  let (cp1, _) := get_at (gid_to_idx gid) 0 regsdata in
-  let (cp2, _) := get_at (gid_to_idx gid + 1) 0 regsdata in
-  (cp1, cp2).
+  Definition delete_thread_regs_from_regs_state: list thread_vt -> regs -> regs :=
+    List.fold_left (fun r t => (* get regs_id from thread, delete it from r *)
+                      match t with
+                        (_, ri, _) => Regs.delete ri r end).
+  Definition delete_best_regs_from_regs_state (best:option leaf_vt) (r:regs) : regs :=
+    match best with
+    | Some (_, ri) => Regs.delete ri r
+    | None => r
+    end.
 
-Definition all_ris (s_vt: pike_vm_state_vt) : list regs_id :=
-  match s_vt with
-  | PVS_vt _ act (Some leaf) blo _ _ _ =>
-      (map ri_of act) ++ [(match leaf with (_, ri) => ri end)] ++ (map ri_of blo)
-  | PVS_vt _ act None blo _ _ _ =>
-      (map ri_of act) ++ (map ri_of blo)
-  | PVS_final_vt (Some leaf) _ => match leaf with (_, ri) => [ri] end
-  | PVS_final_vt None _ => []
-  end.
+  (* small-step semantics for the PikeVM_VT algorithm *)
+  (* Unanchored PikeVM rules are removed: pvs_acc, pvs_nextchar_generate, pvs_next_char_filter *)
+  Inductive pike_vm_step_vt (c:code): pike_vm_state_vt -> pike_vm_state_vt -> Prop :=
+  | pvs_final_vt:
+    (* moving to a final state when there are no more active or blocked threads *)
+    forall inp best seen regs,
+      pike_vm_step_vt c (PVS_vt inp [] best [] None seen regs) (PVS_final_vt best regs)
+  | pvs_end_vt:
+    (* when the list of active is empty and we've reached the end of string *)
+    (* in practice, this rule is never used because we can have no blocked threads *)
+    (* when there is no input left. We keep this rule for convenience in the proofs *)
+    (* and for relating it to the functional version *)
+    forall inp best thr blocked nextprefix seen regs regs'
+           (ADVANCE: advance_input inp forward = None)
+           (DELETE_REGS: regs' = delete_thread_regs_from_regs_state (thr::blocked) regs),
+      pike_vm_step_vt c (PVS_vt inp [] best (thr::blocked) nextprefix seen regs)
+        (PVS_final_vt best regs')
+  | pvs_nextchar_vt:
+    (* when the list of active threads is empty (but not blocked), restart from the blocked ones, proceeding to the next character *)
+    (* reset the set of seen pcs *)
+    forall inp1 inp2 best thr blocked seen regs
+           (ADVANCE: advance_input inp1 forward = Some inp2),
+      pike_vm_step_vt c (PVS_vt inp1 [] best (thr::blocked) None seen regs)
+        (PVS_vt inp2 (thr::blocked) best [] None initial_seenpcs regs)
+  | pvs_skip_vt:
+    (* when the pc has already been seen at this current index, we skip it entirely *)
+    forall inp t active best blocked nextprefix seen regs regs'
+           (SEEN: seen_thread_vt seen t = true)
+           (DELETE_REG:  regs' = delete_thread_regs_from_regs_state [t] regs), (* t is killed, so its regs are deleted *)
+      pike_vm_step_vt c (PVS_vt inp (t::active) best blocked nextprefix seen regs)
+        (PVS_vt inp active best blocked nextprefix seen regs')
+  | pvs_active_vt:
+    (* generated new active threads: add them in front of the low-priority ones *)
+    forall inp t active best blocked nextprefix seen nextactive regs regs'
+           (UNSEEN: seen_thread_vt seen t = false)
+           (STEP: epsilon_step_vt t c inp regs = (EpsActive_vt nextactive, regs')), (* returns next regs *)
+      pike_vm_step_vt c (PVS_vt inp (t::active) best blocked nextprefix seen regs)
+        (PVS_vt inp (nextactive++active) best blocked nextprefix (add_thread_vt seen t) regs')
+  | pvs_match_vt:
+    (* a match is found, discard remaining low-priority active threads *)
+    forall inp t active best blocked nextprefix seen regs regs' regs''
+           (UNSEEN: seen_thread_vt seen t = false)
+           (STEP: epsilon_step_vt t c inp regs = (EpsMatch_vt, regs'))
+           (* delete regs of active threads (except t) and of previous best match *)
+           (DELETE_REGS: regs'' = delete_thread_regs_from_regs_state active
+                                    (delete_best_regs_from_regs_state best regs')),
+      pike_vm_step_vt c (PVS_vt inp (t::active) best blocked nextprefix seen regs) 
+        (PVS_vt inp [] (Some (inp,ri_of t)) blocked None (add_thread_vt seen t) regs'')
+  | pvs_blocked_vt:
+    (* add the new blocked thread after the previous ones *)
+    forall inp t active best blocked nextprefix seen newt regs regs'
+           (UNSEEN: seen_thread_vt seen t = false)
+           (STEP: epsilon_step_vt t c inp regs = (EpsBlocked_vt newt, regs')), (* returns new regs *)
+      pike_vm_step_vt c (PVS_vt inp (t::active) best blocked nextprefix seen regs)
+        (PVS_vt inp active best (blocked ++ [newt]) nextprefix (add_thread_vt seen t) regs').
 
-Definition gm_vt_equiv (gm: group_map) (ri: regs_id) (r: regs) : Prop :=
-  match Regs.get_compressed_data ri r with
-  | None => gm = GroupMap.empty (* assuming groupmap is empty when no updates have been made *)
-  | Some (regsdata) =>
-      forall gid, gm_regs_vals gid gm = vt_regs_vals gid regsdata
-  end.
+  Definition trc_pike_vm_vt (c:code) := @trc pike_vm_state_vt (pike_vm_step_vt c).
 
-Definition leaves_equiv (res: option leaf) (res_vt: option leaf_vt) (r:regs) : Prop :=
-  match res, res_vt with
-  | None, None => True
-  | Some (inp, gm), Some (inp_vt, ri) => inp = inp_vt /\ gm_vt_equiv gm ri r
-  |_, _ => False
-  end.
+  (** * Equivalence to the original PikeVM *)
 
-Definition thread_equiv (t: thread) (t_vt: thread_vt) (r: regs) : Prop :=
-  match t, t_vt with
-    (l, gm, b), (l_vt, ri, b_vt) => l = l_vt /\ gm_vt_equiv gm ri r /\ b = b_vt
-  end.
+  (*** * Defining equivalence *)
 
-Definition threads_equiv (t: list thread) (t_vt: list thread_vt) (r: regs): Prop :=
-  List.Forall2 (fun t t_vt => thread_equiv t t_vt r) t t_vt.
+  Definition gm_regs_vals (gid: group_id) (gm: group_map) : option nat * option nat :=
+    match GroupMap.find gid gm with
+    | None => (None, None)
+    | Some (GroupMap.Range v None) => (Some v, None)
+    | Some (GroupMap.Range o (Some c)) => (Some o, Some c)
+    end.
 
-(* TODO redefine as inductive *)
-Definition state_equiv (s: pike_vm_state) (s_vt: pike_vm_state_vt) : Prop :=
-  match s, s_vt with
-  | PVS i act best blo np seen, PVS_vt i' act' best' blo' np' seen' r =>
-      i = i' /\ np = np' /\ seen = seen' /\
-        threads_equiv act act' r /\ threads_equiv blo blo' r /\ leaves_equiv best best' r
-  | PVS_final best, PVS_final_vt best' r => leaves_equiv best best' r
-  | _, _ => False
-  end.
+  Definition vt_regs_vals (gid: group_id) (regsdata: RegsData.t) : option nat * option nat :=
+    let (cp1, _) := get_at (gid_to_idx gid) 0 regsdata in
+    let (cp2, _) := get_at (gid_to_idx gid + 1) 0 regsdata in
+    (cp1, cp2).
 
-Definition leaf_ids_of (s: pike_vm_state_vt) : list nat :=
-  match s with
-  | PVS_vt _ _ _ _ _ _ r => Regs.get_all_ids (Regs.tree r)
-  | PVS_final_vt _ r => Regs.get_all_ids (Regs.tree r)
-  end.
+  Definition all_ris (s_vt: pike_vm_state_vt) : list regs_id :=
+    match s_vt with
+    | PVS_vt _ act (Some leaf) blo _ _ _ =>
+        (map ri_of act) ++ [(match leaf with (_, ri) => ri end)] ++ (map ri_of blo)
+    | PVS_vt _ act None blo _ _ _ =>
+        (map ri_of act) ++ (map ri_of blo)
+    | PVS_final_vt (Some leaf) _ => match leaf with (_, ri) => [ri] end
+    | PVS_final_vt None _ => []
+    end.
 
-Lemma pike_vm_step_vt_threads_are_leaves :
-  forall c s_vt s_vt',
-    (* s_vt = (PVS inp act_vt best_vt blo_vt None seen regs) *)
-    all_ris s_vt = leaf_ids_of s_vt ->
-    pike_vm_step_vt c s_vt s_vt' ->
-    all_ris s_vt' = leaf_ids_of s_vt'.
-Proof.
-  intros c s_vt s_vt' ALLIDS STEP.
-  dependent induction STEP; simpl in *.
-  - destruct best; simpl in *; auto.
-    destruct l as [_ ri]; repeat constructor.
-    assumption.
-  - destruct best; simpl in *.
-    destruct l as [_ ri].
-    + admit.
-    + admit.
-  - destruct best; simpl in *.
-    destruct l as [_ ri].
-    + admit. (*List property*)
-    + rewrite app_nil_r.
+  Definition gm_vt_equiv (gm: group_map) (ri: regs_id) (r: regs) : Prop :=
+    match Regs.get_compressed_data ri r with
+    | None => gm = GroupMap.empty (* assuming groupmap is empty when no updates have been made *)
+    | Some (regsdata) =>
+        forall gid, gm_regs_vals gid gm = vt_regs_vals gid regsdata
+    end.
+
+  Inductive leaves_equiv : option leaf -> option leaf_vt -> regs -> Prop :=
+  | no_match_equiv: forall r, leaves_equiv None None r
+  | match_equiv:
+    forall inp gm ri r
+           (GMVT: gm_vt_equiv gm ri r),
+      leaves_equiv (Some (inp, gm)) (Some (inp, ri)) r.
+
+  Inductive thread_equiv : thread -> thread_vt -> regs -> Prop :=
+  | thread_eq:
+    forall l b gm ri r
+           (GMVT: gm_vt_equiv gm ri r),
+      thread_equiv (l, gm, b) (l, ri, b) r.
+
+  Definition threads_equiv (t: list thread) (t_vt: list thread_vt) (r: regs): Prop :=
+    List.Forall2 (fun t t_vt => thread_equiv t t_vt r) t t_vt.
+
+  Inductive state_equiv: pike_vm_state -> pike_vm_state_vt -> Prop :=
+  | pvs_state_equiv:
+    forall inp act act_vt best best_vt blo blo_vt np seen r
+           (EQUIV_ACT: threads_equiv act act_vt r)
+           (EQUIV_LEA: leaves_equiv best best_vt r)
+           (EQUIV_BLO: threads_equiv blo blo_vt r),
+      state_equiv (PVS inp act best blo np seen) (PVS_vt inp act_vt best_vt blo_vt np seen r)
+  | pvs_final_state_equiv:
+    forall best best_vt r
+           (EQUIV_LEA: leaves_equiv best best_vt r),
+      state_equiv (PVS_final best) (PVS_final_vt best_vt r).
+
+  (*** * Helpers: EpsMatch and EpsBlock do not modify the register state *)
+
+  Lemma epsmatch_same_regs :
+    forall c inp t_vt r r',
+      epsilon_step_vt t_vt c inp r = (EpsMatch_vt, r') ->
+      r = r'.
+  Proof.
+    intros c inp t_vt r r' H.
+    unfold epsilon_step_vt in *.
+    destruct t_vt as [[l_vt ri] b_vt].
+    destruct (get_pc c l_vt) eqn:BC.
+    - destruct b eqn:B;
+        try (injection H as H1 H2; inversion H1).
+      + injection H as H. assumption.
+      + destruct (check_read rer c0 inp forward); injection H as H1 H2; inversion H1.
+      + destruct (anchor_satisfied rer a inp); injection H as H1 H2; inversion H1.
+      + destruct (close_thread_vt (l_vt, ri, b_vt) g (idx inp) r); injection H as H1 H2; inversion H1.
+      + destruct b_vt; injection H as H _; inversion H.
+    - injection H as H1 H2. inversion H1.
+  Qed.
+
+  Lemma epsblocked_same_regs :
+    forall c inp t_vt t_vt' r r',
+      epsilon_step_vt t_vt c inp r = (EpsBlocked_vt t_vt', r') ->
+      r = r' /\ t_vt' = block_thread_vt t_vt.
+  Proof.
+    intros c inp t_vt t_vt' r r' H.
+    unfold epsilon_step_vt in *.
+    destruct t_vt as [[l_vt ri] b_vt].
+    destruct (get_pc c l_vt) eqn:BC.
+    - destruct b eqn:B;
+        try (injection H as H1 H2; inversion H1).
+      + destruct (check_read rer c0 inp forward); injection H as H1 H2; inversion H1.
+        unfold block_thread_vt.
+        auto.
+      + destruct (anchor_satisfied rer a inp); injection H as H1 H2; inversion H1.
+      + destruct (close_thread_vt (l_vt, ri, b_vt) g (idx inp) r); injection H as H1 H2; inversion H1.
+      + destruct b_vt; injection H as H _; inversion H.
+    - injection H as H1 H2. inversion H1.
+  Qed.
+
+  Lemma epsblocked_orig :
+    forall c inp t t',
+      epsilon_step rer t c inp = EpsBlocked t' ->
+      t' = block_thread t.
+  Proof.
+    intros c inp t t' H.
+    unfold epsilon_step in *.
+    destruct t as [[l gm] b].
+    destruct (get_pc c l) eqn:BC.
+    - destruct b0 eqn:B; try inversion H.
+      + destruct (check_read rer c0 inp forward); try inversion H.
+        congruence.
+      + destruct (anchor_satisfied rer a inp); inversion H.
+      + destruct b; inversion H.
+    - inversion H.
+  Qed.
+
+  (*** * Invariant: register state is valid *)
+
+  Lemma fold_left_preserves {A} {B} :
+    forall (l: list A) (acc: B) P f,
+      P acc ->
+      (forall a x, P a -> In x l -> P (f a x)) ->
+      P (fold_left f l acc).
+  Proof.
+    induction l as [|x xs IH]; intros acc P f H H'; simpl in *.
+    - assumption.
+    - apply IH.
+      + apply H'; auto.
+      + intros a x' HP Hin.
+        apply H'; auto.
+  Qed.
+
+  Inductive state_valid_regs: pike_vm_state_vt -> Prop :=
+  | pvs_valid_regs:
+    forall inp act best blo np seen regs
+           (VALID_REGS: Regs.is_valid_state regs),
+      state_valid_regs (PVS_vt inp act best blo np seen regs)
+  | pvs_final_valid_regs:
+    forall best regs
+           (VALID_REGS: Regs.is_valid_state regs),
+      state_valid_regs (PVS_final_vt best regs).
+
+  Lemma epsactive_valid_regs :
+    forall c inp t tl r r',
+      Regs.is_valid_state r ->
+      epsilon_step_vt t c inp r = (EpsActive_vt tl, r') ->
+      Regs.is_valid_state r'.
+  Proof.
+    intros c inp t tl r r' VALID STEP.
+    unfold epsilon_step_vt in *.
+    destruct t as [[l ri] b].
+    destruct (get_pc c l) eqn:BC.
+    - destruct b0 eqn:B;
+        try (injection STEP as H1 H2; inversion H1); subst.
+      + destruct (check_read rer c0 inp forward); injection STEP as H1 H2.
+        * inversion H1.
+        * subst.
+          apply Regs.delete_valid.
+          assumption.
+      + destruct (anchor_satisfied rer a inp); injection STEP as H1 H2; subst;
+          try apply Regs.delete_valid; assumption.
+      + assumption.
+      + apply Regs.split_valid.
+        assumption.
+      + apply Regs.insert_valid.
+        * admit. (* TODO prove inserted data is valid *)
+        * assumption.
+      + unfold close_thread_vt in *.
+        destruct (Regs.get_compressed_data ri r) eqn:COMP.
+        * destruct (get_at (gid_to_idx g) 0 t0) eqn:GA.
+          destruct o eqn:O;
+            try (injection STEP as H1 H2; subst; assumption).
+          destruct (n <=? idx inp);
+            injection STEP as H1 H2; subst;
+            repeat try apply Regs.insert_valid;
+            try assumption.
+          all: admit. (* TODO prove inserted data is valid *)
+        * injection STEP as H1 H2; subst; assumption.
+      + apply fold_left_preserves; try assumption.
+        intros a x Hv Hin.
+        repeat apply Regs.insert_valid; try assumption.
+        all: admit. (* TODO prove inserted data is valid *)
+      + assumption.
+      + destruct b; injection STEP as H1 H2; subst;
+          try apply Regs.delete_valid; assumption.
+      + apply Regs.delete_valid; assumption.
+    - injection STEP as H1 H2; subst.
+      apply Regs.delete_valid; assumption.
+  Admitted.
+
+  Lemma pike_vm_step_vt_valid_regs :
+    forall c s_vt s_vt',
+      (* s_vt = (PVS inp act_vt best_vt blo_vt None seen regs) *)
+      state_valid_regs s_vt ->
+      pike_vm_step_vt c s_vt s_vt' ->
+      state_valid_regs s_vt'.
+  Proof.
+    intros c s_vt s_vt' H STEP.
+    dependent induction STEP; inversion H; subst; constructor.
+    - assumption.
+    - unfold delete_thread_regs_from_regs_state.
+      apply fold_left_preserves; try assumption.
+      intros a x Hs Hin.
+      destruct x as [[l ri] b].
+      apply Regs.delete_valid.
       assumption.
-  - destruct best; simpl in *.
-    + destruct l as [_ ri].
-      admit. (*use VT prop*)
-    + admit. (*use VT prop*)
-  - destruct best; simpl in *.
-    all: admit.
-  - admit.
-  - admit.
-Admitted.
-
-    
-Lemma pike_vm_step_vt_distinct_ri :
-  forall c s_vt s_vt',
-    (* s_vt = (PVS inp act_vt best_vt blo_vt None seen regs) *)
-    NoDup (all_ris s_vt) ->
-    pike_vm_step_vt c s_vt s_vt' ->
-    NoDup (all_ris s_vt').
-Proof.
-  intros c s_vt s_vt' DISTINCT STEP.
-  dependent induction STEP.
-  - destruct best; simpl in *; auto.
-    destruct l as [_ ri]; repeat constructor.
-    apply in_nil.
-  - destruct best; simpl in *; try constructor.
-    destruct l as [_ ri]; repeat constructor.
-    apply in_nil.
-  - destruct best; simpl in *.
-    + destruct l as [_ ri].
-      admit. (*just some list lemma *)
-    + rewrite app_nil_r. assumption.
-  - destruct best; simpl in *.
-Abort. (* provable but not very useful *)
-
-Lemma seen_equiv : forall t t_vt seen r,
-    thread_equiv t t_vt r ->
-    seen_thread_vt seen t_vt = seen_thread seen t.
-Proof.
-  intros t t_vt seen r H.
-  unfold thread_equiv in *.
-  unfold seen_thread, seen_thread_vt in *.
-  destruct t as [[l gm] b].
-  destruct t_vt as [[l_vt ri] b_vt].
-  destruct H as [Hl [Hr Hb]].
-  subst.
-  reflexivity.
-Qed.
-
-Lemma add_equiv_threads_to_seen : forall t t_vt seen r,
-    thread_equiv t t_vt r ->
-    add_thread seen t = add_thread_vt seen t_vt.
-Proof.
-  unfold add_thread, add_thread_vt.
-  intros t t_vt seen r H.
-  destruct t as [[l gm] b].
-  destruct t_vt as [[l_vt ri] b_vt].
-  destruct H as [Hl [Hr Hb]].
-  subst.
-  reflexivity.
-Qed.
-
-Lemma epsilon_step_equiv_active :
-  forall c inp t t_vt nextactive_vt r r',
-    thread_equiv t t_vt r ->
-    epsilon_step_vt t_vt c inp r = (EpsActive_vt nextactive_vt, r') ->
-    (exists nextactive,
-        epsilon_step rer t c inp = EpsActive nextactive /\
-          threads_equiv nextactive nextactive_vt r').
-Proof.
-  intros c inp t t_vt nextactive_vt r r' Heq H.
-  unfold epsilon_step_vt, epsilon_step, thread_equiv in *.
-  destruct t_vt as [[l_vt ri] b_vt].
-  destruct t as [[l gm] b].
-  destruct Heq as [Hl [Hr Hb]]. subst.
-  destruct (get_pc c l_vt) eqn:BC.
-  - destruct b eqn:B;
-      try (injection H as H1 H2; inversion H1); subst.
-    + destruct (check_read rer c0 inp forward); injection H as H1 H2; inversion H1.
-      subst.
-      exists [].
-      split; [reflexivity | constructor].
-    + destruct (anchor_satisfied rer a inp); injection H as H1 H2; inversion H1; subst.
-      * admit.
-      * exists [].
-        split; [reflexivity | constructor].
-    + exists ([upd_label (l_vt, gm, b_vt) l]).
-      split; try reflexivity.
-      repeat constructor.
+    - assumption.
+    - simpl.
+      destruct t0 as [[l ri] b].
+      apply Regs.delete_valid.
       assumption.
-    + exists ([upd_label (l_vt, gm, b_vt) l; upd_label (l_vt, gm, b_vt) l0]).
-      split; try reflexivity.
-      repeat constructor.
+    - apply epsactive_valid_regs in STEP; try assumption.
+    - apply epsmatch_same_regs in STEP. subst.
+      unfold delete_best_regs_from_regs_state.
+      destruct best;
+        unfold delete_thread_regs_from_regs_state;
+        apply fold_left_preserves; try assumption;
+        try destruct l as [i l]; try (intros a x Hs Hin; destruct x as [[l' ri] b]);
+        apply Regs.delete_valid; assumption.
+    - apply epsblocked_same_regs in STEP. destruct STEP as [Hr Hnewt]. subst.
+      assumption.
+  Qed.
+
+  Lemma init_state_valid_regs :
+    forall inp,
+      state_valid_regs (pike_vm_initial_state_vt inp rer_to_regs_size).
+  Proof.
+    intros inp.
+    unfold pike_vm_initial_state_vt.
+    constructor.
+    unfold Regs.initial_tree, Regs.is_valid_state. simpl.
+    unfold Regs.is_valid_tree_ids. unfold Regs.get_all_ids.
+    repeat split; try tauto.
+    constructor; auto.
+    constructor.
+  Qed.
+
+  (*** * Invariant: register state's leaves ids is a permutation of state's regs_ids *)
+
+  Definition leaf_ids_of (s: pike_vm_state_vt) : list nat :=
+    match s with
+    | PVS_vt _ _ _ _ _ _ r => Regs.get_all_ids (Regs.tree r)
+    | PVS_final_vt _ r => Regs.get_all_ids (Regs.tree r)
+    end.
+  
+  Lemma pike_vm_step_vt_threads_are_leaves :
+    forall c s_vt s_vt',
+      (* s_vt = (PVS inp act_vt best_vt blo_vt None seen regs) *)
+      all_ris s_vt = leaf_ids_of s_vt ->
+      pike_vm_step_vt c s_vt s_vt' ->
+      Permutation (all_ris s_vt') (leaf_ids_of s_vt').
+  Proof.
+    intros c s_vt s_vt' ALLIDS STEP.
+    dependent induction STEP; simpl in *.
+    - destruct best; simpl in *;
+        try destruct l as [_ ri]; rewrite ALLIDS;
+        apply Permutation_refl.
+    - destruct best; simpl in *; destruct thr as [[l' ri] b].
+      + destruct l.
+        admit.
+      + admit.
+    - destruct best; simpl in *.
+      + destruct l.
+        rewrite <- ALLIDS.
+        rewrite app_comm_cons. apply Permutation_app_comm.
+      + rewrite app_nil_r. rewrite ALLIDS.
+        apply Permutation_refl.
+    - destruct best; simpl in *; destruct t0 as [[l' ri] b].
+      + destruct l.
+        admit.
+      + admit.
+    - destruct best; simpl in *.
       all: admit.
-    + exists ([open_thread (l_vt, gm, b_vt) g (idx inp)]).
-      split; try reflexivity.
-      repeat constructor.
+    - apply epsmatch_same_regs in STEP. subst.
       admit.
-    + exists ([close_thread (l_vt, gm, b_vt) g (idx inp)]).
-      split; try reflexivity.
-      repeat constructor.
-      admit.
-    + exists ([reset_thread (l_vt, gm, b_vt) l]).
-      split; try reflexivity.
-      repeat constructor.
-      admit.
-    + exists ([begin_thread (l_vt, gm, b_vt)]).
-      split; try reflexivity.
-      repeat constructor.
-      assumption.
-    + destruct b_vt; injection H as H1 H2; inversion H1; subst.
-      * exists ([upd_label (l_vt, gm, CanExit) l]).
+    - apply epsblocked_same_regs in STEP. destruct STEP as [Hr Hnewt]. subst.
+      destruct best; simpl in *;
+        try destruct l;
+        rewrite <- ALLIDS;
+        destruct t0 as [[l ri] b];
+        rewrite map_app; simpl;
+        try rewrite app_assoc with (m:= r :: map ri_of blocked) (n:= [ri]);
+        try rewrite app_assoc with (m:= map ri_of blocked) (n:= [ri]);
+        apply Permutation_app_comm.
+  Admitted.
+
+  Lemma init_state_threads_are_leaves :
+    forall inp,
+      let si := pike_vm_initial_state_vt inp rer_to_regs_size in
+      Permutation (all_ris si) (leaf_ids_of si).
+  Proof.
+    intros inp; simpl.
+    unfold vt_initial_id.
+    repeat constructor.
+  Qed.
+
+  (*** * Equivalence invariant *)
+
+  Lemma seen_equiv : forall t t_vt seen r,
+      thread_equiv t t_vt r ->
+      seen_thread_vt seen t_vt = seen_thread seen t.
+  Proof.
+    intros t t_vt seen r H.
+    inversion H. subst.
+    unfold seen_thread, seen_thread_vt in *.
+    reflexivity.
+  Qed.
+
+  Lemma add_equiv_threads_to_seen : forall t t_vt seen r,
+      thread_equiv t t_vt r ->
+      add_thread seen t = add_thread_vt seen t_vt.
+  Proof.
+    unfold add_thread, add_thread_vt.
+    intros t t_vt seen r H.
+    inversion H. subst.
+    reflexivity.
+  Qed.
+
+  Lemma epsilon_step_equiv_active :
+    forall c inp t t_vt nextactive_vt r r',
+      thread_equiv t t_vt r ->
+      epsilon_step_vt t_vt c inp r = (EpsActive_vt nextactive_vt, r') ->
+      (exists nextactive,
+          epsilon_step rer t c inp = EpsActive nextactive /\
+            threads_equiv nextactive nextactive_vt r').
+  Proof.
+    intros c inp t t_vt nextactive_vt r r' Heq H.
+    inversion Heq. subst.
+    unfold epsilon_step_vt, epsilon_step in *.
+    destruct (get_pc c l) eqn:BC.
+    - destruct b0 eqn:B;
+        try (injection H as H1 H2; inversion H1); subst.
+      + destruct (check_read rer c0 inp forward); injection H as H1 H2; inversion H1.
+        subst.
+        exists [].
+        split; [reflexivity | constructor].
+      + destruct (anchor_satisfied rer a inp); injection H as H1 H2; inversion H1; subst.
+        * admit.
+        * exists [].
+          split; [reflexivity | constructor].
+      + exists ([upd_label (l, gm, b) l0]).
         split; try reflexivity.
         repeat constructor.
         assumption.
-      * exists [].
+      + exists ([upd_label (l, gm, b) l0; upd_label (l, gm, b) l0]).
+        split; try reflexivity.
+        repeat constructor.
+        all: admit.
+      + exists ([open_thread (l, gm, b) g (idx inp)]).
+        split; try reflexivity.
+        repeat constructor.
+        admit.
+      + exists ([close_thread (l, gm, b) g (idx inp)]).
+        split; try reflexivity.
+        repeat constructor.
+        admit.
+      + exists ([reset_thread (l, gm, b) l0]).
+        split; try reflexivity.
+        repeat constructor.
+        admit.
+      + exists ([begin_thread (l, gm, b)]).
+        split; try reflexivity.
+        repeat constructor.
+        assumption.
+      + destruct b; injection H as H1 H2; inversion H1; subst.
+        * exists ([upd_label (l, gm, CanExit) l0]).
+          split; try reflexivity.
+          repeat constructor.
+          assumption.
+        * exists [].
+          split; [reflexivity | constructor].
+      + exists [].
         split; [reflexivity | constructor].
-    + exists [].
-      split; [reflexivity | constructor].
-  - injection H as H1 H2. inversion H1. subst.
-    exists [].
-    split.
-    + reflexivity.
-    + constructor.
-Admitted.
+    - injection H as H1 H2. inversion H1. subst.
+      exists [].
+      split.
+      + reflexivity.
+      + constructor.
+  Admitted.
 
-Lemma epsilon_step_equiv_match :
-  forall c inp t t_vt r r',
-    thread_equiv t t_vt r ->
-    epsilon_step_vt t_vt c inp r = (EpsMatch_vt, r') ->
-    epsilon_step rer t c inp = EpsMatch /\ r = r'.
-Proof.
-  intros c inp t t_vt r r' Heq H.
-  unfold epsilon_step_vt, epsilon_step, thread_equiv in *.
-  destruct t_vt as [[l_vt ri] b_vt].
-  destruct t as [[l gm] b].
-  destruct Heq as [Hl [Hr Hb]]. subst.
-  destruct (get_pc c l_vt) eqn:BC.
-  - destruct b eqn:B;
-      try (injection H as H1 H2; inversion H1).
-    + injection H as H. subst.
-      auto.
-    + destruct (check_read rer c0 inp forward); injection H as H1 H2; inversion H1.
-    + destruct (anchor_satisfied rer a inp); injection H as H1 H2; inversion H1.
-    + destruct b_vt; injection H as H _; inversion H.
-  - injection H as H1 H2. inversion H1.
-Qed.
-
-Lemma epsilon_step_equiv_blocked :
-  forall c inp t t_vt newt_vt r r',
-    thread_equiv t t_vt r ->
-    epsilon_step_vt t_vt c inp r = (EpsBlocked_vt newt_vt, r') ->
-    (exists newt,
-        epsilon_step rer t c inp = EpsBlocked newt /\
-          thread_equiv newt newt_vt r') /\ r = r'.
-Proof.
-  intros c inp t t_vt newt_vt r r' Heq H.
-  unfold epsilon_step_vt, epsilon_step, thread_equiv in *.
-  destruct t_vt as [[l_vt ri] b_vt].
-  destruct t as [[l gm] b].
-  destruct Heq as [Hl [Hr Hb]]. subst.
-  destruct (get_pc c l_vt) eqn:BC.
-  - destruct b eqn:B;
-      try (injection H as H1 H2; inversion H1).
-    + destruct (check_read rer c0 inp forward);
-        injection H as H1 H2.
-      * split; try assumption.
-        subst.
-        exists (l_vt + 1, gm, CanExit).
+  Lemma epsilon_step_equiv_match :
+    forall c inp t t_vt r r',
+      thread_equiv t t_vt r ->
+      epsilon_step_vt t_vt c inp r = (EpsMatch_vt, r') ->
+      epsilon_step rer t c inp = EpsMatch.
+  Proof.
+    intros c inp t t_vt r r' Heq H.
+    unfold epsilon_step_vt, epsilon_step in *.
+    inversion Heq. subst.
+    destruct (get_pc c l) eqn:BC.
+    - destruct b0 eqn:B;
+        try (injection H as H1 H2; inversion H1).
+      + injection H as H. subst.
         auto.
-      * inversion H1.
-    + destruct (anchor_satisfied rer a inp); injection H as H1 H2; inversion H1.
-    + destruct b_vt; injection H as H _; inversion H.
-  - injection H as H1 H2. inversion H1.
-Qed.
+      + destruct (check_read rer c0 inp forward); injection H as H1 H2; inversion H1.
+      + destruct (anchor_satisfied rer a inp); injection H as H1 H2; inversion H1.
+      + destruct (close_thread_vt (l, ri, b) g (idx inp) r).
+        injection H as H1 H2; inversion H1.
+      + destruct b; injection H as H _; inversion H.
+    - injection H as H1 H2. inversion H1.
+  Qed.
 
-Lemma pike_vm_step_vt_equiv :
-  forall c s s_vt s' s_vt',
-    (* s = (PVS inp act best blo None seen) *)
-    (* s_vt = (PVS inp act_vt best_vt blo_vt None seen regs) *)
-    state_equiv s s_vt ->
-    pike_vm_step rer c s s' ->
-    pike_vm_step_vt c s_vt s_vt' ->
-    state_equiv s' s_vt'.
-Proof.
-  unfold state_equiv.
-  intros c s s_vt s' s_vt' H STEP STEPVT.
-  dependent induction STEPVT; destruct s; try contradiction.
-  - (* pvs_final_vt *)
-    destruct H as [Hinp [Hnp [Hs [EQUIV_ACT [EQUIV_BLO EQUIV_LEA]]]]].
-    destruct active as [| t act]; inversion EQUIV_ACT; subst.
-    destruct blocked as [| t blo]; inversion EQUIV_BLO; subst.
-    inversion STEP. subst.
-    assumption.
-  - (* pvs_end_vt *)
-    destruct H as [Hinp [Hnp [Hs [EQUIV_ACT [EQUIV_BLO EQUIV_LEA]]]]].
-    destruct active as [| t act]; inversion EQUIV_ACT; subst.
-    destruct blocked0 as [| t blo]; inversion EQUIV_BLO; subst.
-    inversion STEP; subst; try congruence.
-    admit.
-  - (* pvs_nextchar_vt *)
-    destruct H as [Hinp [Hnp [Hs [EQUIV_ACT [EQUIV_BLO EQUIV_LEA]]]]].
-    inversion EQUIV_ACT. subst.
-    inversion EQUIV_BLO. subst.
-    inversion STEP; subst.
-    + congruence.
-    + repeat split; try assumption. congruence.
-  - (* pvs_skip_vt *)
-    destruct H as [Hinp [Hnp [Hs [EQUIV_ACT [EQUIV_BLO EQUIV_LEA]]]]].
-    destruct active0 as [| t act]; inversion EQUIV_ACT; subst.
-    apply seen_equiv with (seen:= seen) in H2; auto.
-    inversion STEP; subst; try (rewrite H2 in *; congruence).
-    repeat split; auto.
-    + admit.
-    + admit.
-    + destruct best0, best; try contradiction; try tauto.
-      destruct t0 as [[la0 ri0] b0].
-      unfold leaves_equiv in *. simpl.
-      destruct l as [i gm]. destruct l0 as [i_vt l_vt].
-      split; try tauto.
-      unfold gm_vt_equiv.
+  Lemma epsilon_step_equiv_blocked :
+    forall c inp t t_vt newt_vt r r',
+      thread_equiv t t_vt r ->
+      epsilon_step_vt t_vt c inp r = (EpsBlocked_vt newt_vt, r') ->
+      (exists newt,
+          epsilon_step rer t c inp = EpsBlocked newt /\
+            thread_equiv newt newt_vt r').
+  Proof.
+    intros c inp t t_vt newt_vt r r' Heq H.
+    unfold epsilon_step_vt, epsilon_step in *.
+    inversion Heq. subst.
+    destruct (get_pc c l) eqn:BC.
+    - destruct b0 eqn:B;
+        try (injection H as H1 H2; inversion H1).
+      + destruct (check_read rer c0 inp forward);
+          injection H as H1 H2.
+        * subst.
+          exists (l+1, gm, CanExit).
+          split; try constructor.
+          assumption.
+        * inversion H1.
+      + destruct (anchor_satisfied rer a inp); injection H as H1 H2; inversion H1.
+      + destruct (close_thread_vt (l, ri, b) g (idx inp) r);
+          injection H as H1 H2; inversion H1.
+      + destruct b; injection H as H _; inversion H.
+    - injection H as H1 H2. inversion H1.
+  Qed.
+
+  Lemma pike_vm_step_vt_equiv :
+    forall c s s_vt s' s_vt',
+      (* s = (PVS inp act best blo None seen) *)
+      (* s_vt = (PVS inp act_vt best_vt blo_vt None seen regs) *)
+      state_equiv s s_vt ->
+      pike_vm_step rer c s s' ->
+      pike_vm_step_vt c s_vt s_vt' ->
+      state_equiv s' s_vt'.
+  Proof.
+    intros c s s_vt s' s_vt' H STEP STEPVT.
+    dependent induction STEPVT; destruct s; inversion H; subst.
+    - (* pvs_final_vt *)
+      inversion EQUIV_ACT. inversion EQUIV_BLO. subst.
+      inversion STEP. subst.
+      constructor.
+      assumption.
+    - (* pvs_end_vt *)
+      inversion EQUIV_ACT. inversion EQUIV_BLO. subst.
+      inversion STEP; subst; try congruence.
+      constructor.
       admit.
-  - (* pvs_active_vt *)
-    destruct H as [Hinp [Hnp [Hs [EQUIV_ACT [EQUIV_BLO EQUIV_LEA]]]]].
-    destruct active0 as [| t act]; inversion EQUIV_ACT; subst.
-    specialize (epsilon_step_equiv_active _ _ _ _ _ _ _ H2 STEP0) as STEP1.
-    destruct STEP1 as [na [STEP1 Hna]].
-    apply seen_equiv with (seen:= seen) in H2; auto.
-    inversion STEP; subst; try (rewrite H12 in *; congruence); try congruence.
-    repeat split; auto.
-    + apply add_equiv_threads_to_seen with (r:=regs0).
-      inversion EQUIV_ACT. subst. assumption.
-    + rewrite STEP1 in STEP2. injection STEP2 as STEP2. subst.
-      apply Forall2_app; auto.
-      (* TODO specify in lemma what are exactly the possible values for regs' *)
-      admit.
-    + admit.
-    + admit.
-  - (* pvs_match_vt *)
-    destruct H as [Hinp [Hnp [Hs [EQUIV_ACT [EQUIV_BLO EQUIV_LEA]]]]].
-    destruct active0 as [| t act]; inversion EQUIV_ACT; subst.
-    specialize (epsilon_step_equiv_match _ _ _ _ _ _ H2 STEP0) as [STEP1 Hr].
-    specialize (seen_equiv t t0 seen regs0 H2) as Hse.
-    inversion STEP; subst; try (rewrite H12 in *; congruence); try congruence.
-    repeat split; try reflexivity.
-    + apply add_equiv_threads_to_seen with (r:=regs').
-      inversion EQUIV_ACT. subst. assumption.
-    + constructor.
-    + admit.
-    + unfold thread_equiv in *.
-      admit.
-  - (* pvs_blocked_vt *)
-    destruct H as [Hinp [Hnp [Hs [EQUIV_ACT [EQUIV_BLO EQUIV_LEA]]]]].
-    destruct active0 as [| t act]; inversion EQUIV_ACT; subst.
-    specialize (epsilon_step_equiv_blocked _ _ _ _ _ _ _ H2 STEP0) as [[nt [STEP1 Hnt]] Hr].
-    apply seen_equiv with (seen:= seen) in H2; auto.
-    inversion STEP; subst; try (rewrite H12 in *; congruence); try congruence.
-    repeat split; auto.
-    + apply add_equiv_threads_to_seen with (r:=regs').
-      inversion EQUIV_ACT. subst. assumption.
-    + rewrite STEP1 in STEP2. injection STEP2 as STEP2. subst.
-      apply Forall2_app; auto.
-Admitted.
+    - (* pvs_nextchar_vt *)
+      inversion EQUIV_ACT. inversion EQUIV_BLO. subst.
+      inversion STEP; subst.
+      + congruence.
+      + rewrite ADVANCE in ADVANCE0. injection ADVANCE0 as INP. rewrite INP.
+        constructor; assumption.
+    - (* pvs_skip_vt *)
+      inversion EQUIV_ACT. subst.
+      apply seen_equiv with (seen:= seen) in H3; auto.
+      inversion STEP; subst; try (rewrite H3 in *; congruence).
+      constructor.
+      + admit.
+      + destruct best0, best; inversion EQUIV_LEA; subst; constructor.
+        admit.
+      + admit.
+    - (* pvs_active_vt *)
+      inversion EQUIV_ACT. subst.
+      specialize (epsilon_step_equiv_active _ _ _ _ _ _ _ H3 STEP0) as STEP1.
+      destruct STEP1 as [na [STEP1 Hna]].
+      specialize (seen_equiv _ _ seen regs0 H3) as Hse.
+      specialize (add_equiv_threads_to_seen _ _ seen _ H3) as Hadd.
+      inversion STEP; subst; try (rewrite H12 in *; congruence); try congruence.
+      rewrite Hadd.
+      constructor.
+      + admit.
+      + destruct best0, best; inversion EQUIV_LEA; subst; constructor.
+        admit.
+      + admit.
+    - (* pvs_match_vt *)
+      inversion EQUIV_ACT. subst.
+      specialize (epsilon_step_equiv_match _ _ _ _ _ _ H3 STEP0) as STEP1.
+      specialize (epsmatch_same_regs _ _ _ _ _ STEP0) as Hr.
+      specialize (seen_equiv _ _ seen regs0 H3) as Hse.
+      specialize (add_equiv_threads_to_seen _ _ seen _ H3) as Hadd.
+      inversion STEP; subst; try (rewrite H12 in *; congruence); try congruence.
+      rewrite Hadd.
+      constructor.
+      + constructor.
+      + constructor.
+        admit.
+      + admit.
+    - (* pvs_blocked_vt *)
+      inversion EQUIV_ACT. subst.
+      specialize (epsilon_step_equiv_blocked _ _ _ _ _ _ _ H3 STEP0) as [nt [STEP1 Hnt]].
+      specialize (epsblocked_same_regs _ _ _ _ _ _ STEP0) as [Hr Hnewt].
+      specialize (seen_equiv _ _ seen regs0 H3) as Hse.
+      specialize (add_equiv_threads_to_seen _ _ seen _ H3) as Hadd.
+      inversion STEP; subst; try (rewrite H12 in *; congruence); try congruence.
+      rewrite Hadd.
+      constructor; auto.
+      rewrite STEP2 in *. injection STEP1 as STEP1. subst.
+      apply epsblocked_orig in STEP2. subst.
+      apply Forall2_app; try assumption.
+      constructor; auto.
+  Admitted.
 
-Theorem trc_pikevm_vt_equiv: 
-  forall r s s_vt result result_vt regs,
-    state_equiv s s_vt ->
-    trc_pike_vm rer r s (PVS_final result) ->
-    trc_pike_vm_vt r s_vt (PVS_final_vt result_vt regs) ->
-    leaves_equiv result result_vt regs.
-Proof.
-  intros r s s_vt result result_vt regs EQUIV TRC TRCVT.
-  dependent induction TRC.
-  - unfold state_equiv in EQUIV.
-    destruct s_vt; try contradiction.
-    inversion TRCVT; subst.
-    + assumption.
-    + inversion STEP.
-  - inversion TRCVT. subst.
-    + unfold state_equiv in EQUIV.
-      destruct x; try contradiction.
-      inversion STEP.
-    + eapply IHTRC with (s_vt := y0).
-      * eapply pike_vm_step_vt_equiv; eauto.
-      * reflexivity.
-      * assumption.
-Qed.
+  Lemma init_states_equiv :
+    forall inp,
+      state_equiv (pike_vm_initial_state inp) (pike_vm_initial_state_vt inp rer_to_regs_size).
+  Proof.
+    intro inp.
+    unfold pike_vm_initial_state, pike_vm_initial_state_vt.
+    simpl.
+    repeat split; repeat constructor.
+  Qed.
 
-Lemma init_states_equiv :
-  forall inp,
-    state_equiv (pike_vm_initial_state inp) (pike_vm_initial_state_vt inp rer_to_regs_size).
-Proof.
-  intro inp.
-  unfold pike_vm_initial_state, pike_vm_initial_state_vt.
-  simpl.
-  repeat split; repeat constructor.
-Qed.
+  (*** * Main results *)
 
-Theorem pikevm_vt_equiv: 
-  forall r inp result result_vt regs,
-  trc_pike_vm rer (compilation r) (pike_vm_initial_state inp) (PVS_final result) ->
-  trc_pike_vm_vt (compilation r) (pike_vm_initial_state_vt inp (rer_to_regs_size)) (PVS_final_vt result_vt regs) ->
-  leaves_equiv result result_vt regs.
-Proof.
-  intros r inp result result_vt regs TRC TRCVT.
-  eapply trc_pikevm_vt_equiv.
-  - apply init_states_equiv.
-  - exact TRC.
-  - exact TRCVT.
-Qed.
+  Lemma trc_pikevm_vt_equiv: 
+    forall r s s_vt result result_vt regs,
+      state_equiv s s_vt ->
+      trc_pike_vm rer r s (PVS_final result) ->
+      trc_pike_vm_vt r s_vt (PVS_final_vt result_vt regs) ->
+      leaves_equiv result result_vt regs.
+  Proof.
+    intros r s s_vt result result_vt regs EQUIV TRC TRCVT.
+    dependent induction TRC.
+    - inversion EQUIV. subst.
+      inversion TRCVT; subst.
+      + assumption.
+      + inversion STEP.
+    - inversion TRCVT; subst.
+      + inversion EQUIV. subst.
+        inversion STEP.
+      + eapply IHTRC with (s_vt := y0).
+        * eapply pike_vm_step_vt_equiv; eauto.
+        * reflexivity.
+        * assumption.
+  Qed.
+
+  Theorem pikevm_vt_equiv: 
+    forall r inp result result_vt regs,
+      trc_pike_vm rer (compilation r) (pike_vm_initial_state inp) (PVS_final result) ->
+      trc_pike_vm_vt (compilation r) (pike_vm_initial_state_vt inp (rer_to_regs_size)) (PVS_final_vt result_vt regs) ->
+      leaves_equiv result result_vt regs.
+  Proof.
+    intros r inp result result_vt regs TRC TRCVT.
+    eapply trc_pikevm_vt_equiv.
+    - apply init_states_equiv.
+    - exact TRC.
+    - exact TRCVT.
+  Qed.
 
 End PikeVM_VT.
